\begin{figure}
$ E \rightarrow id $ \\
$ E \rightarrow	lit $ \\
$ E \rightarrow E ^{} E $ \\
$ E \rightarrow	E * E $ \\
$ E \rightarrow	E / E $ \\
$ E \rightarrow E + E $ \\
$ E \rightarrow	E - E $ \\
$ E \rightarrow	E .. E $ \\
$ E \rightarrow	E < E $ \\
$ E \rightarrow	E > E $ \\
$ E \rightarrow	E <= E $ \\
$ E \rightarrow	E >= E $ \\
$ E \rightarrow	E ~= E $ \\
$ E \rightarrow	E == E $ \\
$ E \rightarrow	( E ) $ \\
$ E \rightarrow	id ( E ) $ \\
$ E \rightarrow	id ( P ) $ \\
$ P \rightarrow E, E $ \\
$ P \rightarrow	P, E $ \\
\caption{Pravidla gramatiky výrazů}
\label{syn.expr}
\end{figure}
